

Metric

$$g_{\mu\nu} = e_{\mu} \cdot e_{\nu}$$

$$W = V^{\mu} e_{\mu} \quad ; \quad V^2 = V^{\mu} V^{\nu} e_{\mu} \cdot e_{\nu}$$

$$V^2 = g_{\mu\nu} V^{\mu} V^{\nu} = V^{\mu} V_{\mu}$$

$$V_{\mu} = g_{\mu\nu} V^{\nu}$$

$$dx = dx^{\mu} e_{\mu}$$

$$ds^2 = dx \cdot dx$$

$$ds^2 = g_{\mu\nu} dx^{\mu} dx^{\nu}$$

$$g^{\mu\nu} = (g_{\mu\nu})^{-1}$$

;

$$g_{\mu\nu} g^{\mu\lambda} = \delta_{\nu}^{\lambda}$$

$$\begin{cases} x' = \gamma(x - vt) \\ y' = y \\ z' = z \\ t' = \gamma(t - \frac{vx}{c^2}) \end{cases}$$

$$(X^\mu \rightarrow X^a)$$

$$\gamma = \frac{1}{\sqrt{1 - v^2/c^2}}$$

$$e^a_\mu = \frac{\partial X^a}{\partial X^\mu}$$

$$= \begin{bmatrix} \gamma & -\gamma \frac{v}{c} & 0 & 0 \\ -\gamma \frac{v}{c} & \gamma & 0 & 0 \\ 0 & 0 & 1 & 0 \\ 0 & 0 & 0 & 1 \end{bmatrix}$$

$$\frac{\partial X^{10}}{\partial X} = c \frac{\partial t'}{\partial X} = c \left(-\frac{v}{c^2} \right) \gamma = -\gamma \frac{v}{c}$$

$$ds^2 = g_{ab} dx^a dx^b = g_{\mu\nu} dx^\mu dx^\nu$$

$$= g_{ab} e^a_\mu dx^\mu e^b_\nu dx^\nu = g_{\mu\nu} dx^\mu dx^\nu$$

$$g_{\mu\nu} = e^a_\mu e^b_\nu g_{ab}$$

$$g_{00} = e^a_\alpha e^b_\beta g^{ab} = \gamma e^b_0 g_{0b} + \left(-\frac{\gamma v}{c}\right) e^b_\alpha g_{\alpha b}$$

$$= \gamma^2 g_{00} - \frac{\gamma^2 v}{c} g_{0L} - \frac{\gamma^2 v}{c} g_{L0} + \left(\frac{\gamma v}{c}\right)^2 g_{LL}$$

$$g_{10} = e^a_\alpha e^b_\beta g^{ab} = \gamma e^b_1 g_{0b} + \left(-\frac{\gamma v}{c}\right) e^b_\alpha g_{\alpha b}$$

$$= -\frac{\gamma^2 v}{c} g_{00} + \gamma^2 g_{0L} + \left(\frac{\gamma v}{c}\right)^2 g_{0L} - \frac{\gamma^2 v}{c} g_{LL}$$

$$g_{11} = e^a_\alpha e^b_\beta g^{ab} = -\frac{\gamma v}{c} e^b_1 g_{0b} + \gamma e^b_\alpha g_{\alpha b}$$

$$= \left(\frac{\gamma v}{c}\right)^2 g_{00} - \frac{\gamma^2 v}{c} g_{0L} - \frac{\gamma^2 v}{c} g_{L0} + \gamma^2 g_{LL}$$

$$\left\{ \begin{array}{l} (1-\gamma^2) g_{00} = -2 \frac{\gamma^2 v}{c} g_{0L} + \frac{\gamma^2 v^2}{c^2} g_{LL} \\ (1-\gamma^2 - \frac{\gamma^2 v^2}{c^2}) g_{0L} = \frac{\gamma^2 v}{c} g_{00} - \frac{\gamma^2 v}{c} g_{LL} \\ (1-\gamma^2) g_{LL} = -2 \frac{\gamma^2 v}{c} g_{0L} + \frac{\gamma^2 v^2}{c^2} g_{00} \end{array} \right.$$

$$g_{00} = -g_{11} \quad ; \quad g_{0i} = 0 \quad ; \quad g_{11} = a$$

$$g_{\mu\nu} = \begin{bmatrix} \gamma & -\gamma \frac{v}{c} & 0 & 0 \\ -\gamma \frac{v}{c} & \gamma & 0 & 0 \\ 0 & 0 & 1 & 0 \\ 0 & 0 & 0 & 1 \end{bmatrix} \begin{bmatrix} -a & 0 & 0 & 0 \\ 0 & a & 0 & 0 \\ 0 & 0 & 1 & 0 \\ 0 & 0 & 0 & 1 \end{bmatrix} \begin{bmatrix} \gamma & -\gamma \frac{v}{c} & 0 & 0 \\ -\gamma \frac{v}{c} & \gamma & 0 & 0 \\ 0 & 0 & 1 & 0 \\ 0 & 0 & 0 & 1 \end{bmatrix}$$

$$g_{\mu\nu} = \begin{bmatrix} \gamma & -\gamma \frac{v}{c} & 0 & 0 \\ -\gamma \frac{v}{c} & \gamma & 0 & 0 \\ 0 & 0 & 1 & 0 \\ 0 & 0 & 0 & 1 \end{bmatrix} \begin{bmatrix} -a\gamma & \gamma \frac{av}{c} & 0 & 0 \\ -\gamma \frac{av}{c} & \gamma a & 0 & 0 \\ 0 & 0 & 1 & 0 \\ 0 & 0 & 0 & 1 \end{bmatrix}$$

$$= \begin{bmatrix} -a\gamma^2 + a\gamma^2 \frac{v^2}{c^2} & 0 & 0 & 0 \\ 0 & -\gamma^2 \frac{v^2}{c^2} a + \gamma^2 a & 0 & 0 \\ 0 & 0 & 1 & 0 \\ 0 & 0 & 0 & 1 \end{bmatrix} = \begin{bmatrix} -a & 0 & 0 & 0 \\ 0 & a & 0 & 0 \\ 0 & 0 & 1 & 0 \\ 0 & 0 & 0 & 1 \end{bmatrix}$$

$$ds^2 = -a \, c^2 dt^2 + a \, dx^2 + dy^2 + dz^2 \quad ; \quad a=1$$

$$ds^2 = -c^2 dt^2 + dx^2 + dy^2 + dz^2$$

$$d\tau^2 = - \frac{ds^2}{c^2}$$

$$d\tau^2 = dt^2 \left(1 - \frac{v^2}{c^2} \right) ;$$

$$\tau = \int dt \sqrt{1 - v^2/c^2}$$

$$\eta_{ab} = \begin{bmatrix} -1 & 0 & 0 & 0 \\ 0 & 1 & 0 & 0 \\ 0 & 0 & 1 & 0 \\ 0 & 0 & 0 & 1 \end{bmatrix} ; \text{ Minkowski}$$